Rework ARMv8 to capture more reordering behaviour

ARMv8.thy
@@ -1,75 +1,14 @@
 theory ARMv8
-  imports Syntax Semantics
+  imports ARMv8_State Syntax
 begin
 
 chapter \<open>ARMv8\<close>
-
-section \<open>State Encoding\<close>
-
-type_synonym ('v,'r) state = "(('v \<Rightarrow> 'v) \<times> ('r \<Rightarrow> 'v))"
-type_synonym ('v,'r) pred  = "('v,'r) state \<Rightarrow> bool"
-type_synonym ('v,'r) rpred = "('v \<Rightarrow> 'v) \<Rightarrow> ('v \<Rightarrow> 'v) \<Rightarrow> bool"
-type_synonym ('v,'r) gpred  = "('v \<Rightarrow> 'v) \<Rightarrow> bool"
-
-named_theorems pred_defs
-definition conj  (infixr "\<and>\<^sub>p" 35)
-  where "conj l r \<equiv> \<lambda>m. (l m) \<and> (r m)"
-definition imp  (infixr "\<longrightarrow>\<^sub>p" 35)
-  where "imp l r \<equiv> \<lambda>m. (l m) \<longrightarrow> (r m)"
-definition entail (infix "\<turnstile>\<^sub>p" 25)
-  where "entail P Q \<equiv> \<forall>m. P m \<longrightarrow> Q m"
-definition assert
-  where "assert b \<equiv> \<lambda>m. b"
-declare assert_def [pred_defs]
-declare entail_def [pred_defs]
-declare conj_def [pred_defs]
-declare imp_def [pred_defs]
-definition stabilize 
-  where "stabilize R P \<equiv> \<lambda>m. \<forall>m'. R m m' \<longrightarrow> P m'"
-definition reflexive 
-  where "reflexive R \<equiv> \<forall>m . R m  m"
-definition transitive 
-  where "transitive R \<equiv> \<forall>m m' m''. R m m' \<longrightarrow> R m' m'' \<longrightarrow> R m m''"
-abbreviation PFalse 
-  where "PFalse \<equiv> \<lambda>m. False"
-abbreviation PTrue 
-  where "PTrue \<equiv> \<lambda>m. True"
-
-subsection \<open>Write Operations\<close>
-
-definition pair_upd1 :: "(('v \<Rightarrow> 'v) \<times> ('c \<Rightarrow> 'v)) \<Rightarrow> 'v \<Rightarrow> 'v \<Rightarrow> (('v \<Rightarrow> 'v) \<times> ('c \<Rightarrow> 'v))"
-  where "pair_upd1 f a b = (\<lambda>x. if x = a then b else (fst f) x, snd f)"
-
-definition pair_upd2 :: "(('a \<Rightarrow> 'b) \<times> ('c \<Rightarrow> 'd)) \<Rightarrow> 'c \<Rightarrow> 'd \<Rightarrow> (('a \<Rightarrow> 'b) \<times> ('c \<Rightarrow> 'd))"
-  where "pair_upd2 f a b = (fst f, \<lambda>x. if x = a then b else (snd f) x)"
-
-nonterminal updbinds and updbind
-
-syntax
-  "_updbind1" :: "'a \<Rightarrow> 'a \<Rightarrow> updbind"             ("(2_ :=\<^sub>1/ _)")
-  "_updbind2" :: "'a \<Rightarrow> 'a \<Rightarrow> updbind"             ("(2_ :=\<^sub>2/ _)")
-  ""         :: "updbind \<Rightarrow> updbinds"             ("_")
-  "_updbinds":: "updbind \<Rightarrow> updbinds \<Rightarrow> updbinds" ("_,/ _")
-  "_Update"  :: "'a \<Rightarrow> updbinds \<Rightarrow> 'a"            ("_/'((_)')" [1000, 0] 900)
-
-translations
-  "_Update f (_updbinds b bs)" \<rightleftharpoons> "_Update (_Update f b) bs"
-  "f(x:=\<^sub>1y)" \<rightleftharpoons> "CONST pair_upd1 f x y"
-  "f(x:=\<^sub>2y)" \<rightleftharpoons> "CONST pair_upd2 f x y"
-
-subsection \<open>Read Operations\<close>
-
-abbreviation rg
-  where "rg m r \<equiv> (snd m) r"
-
-abbreviation ld
-  where "ld m x \<equiv> (fst m) x"
 
 section \<open>Sub-Instruction Language Definition\<close>
 
 datatype ('v,'r) exp = Reg 'r | Val 'v | Glb 'v 'v | Exp "'v list \<Rightarrow> 'v" "('v,'r) exp list"
 
-fun ev
+fun ev 
   where 
     "ev m (Reg r) = m r" | 
     "ev _ (Val v) = v" |
@@ -82,11 +21,11 @@ fun deps
     "deps (Exp _ rs) = \<Union>(deps ` set rs)" |
     "deps _ = {}"
 
-fun addrs
+fun addr
   where
-    "addrs (Glb _ v) = {v}" |
-    "addrs (Exp _ rs) = \<Union>(addrs ` set rs)" |
-    "addrs _ = {}"
+    "addr (Glb _ v) = {v}" |
+    "addr (Exp _ rs) = \<Union>(addr ` set rs)" |
+    "addr _ = {}"
 
 fun subst
   where
@@ -94,94 +33,128 @@ fun subst
     "subst (Exp f rs) r e = (Exp f (map (\<lambda>x. subst x r e) rs))" |
     "subst e _ _ = e"
 
+type_synonym ('v,'r,'a) aux = "('v,'r,'a) tstate_scheme \<Rightarrow> 'a"
+
 text \<open>Capture a simple set of sub-instructions, covering memory operations and fences\<close>
-datatype ('v,'r) inst =
-    load 'v "('v,'r) exp"
-  | store 'v "('v,'r) exp"
+datatype ('v,'r,'a) inst =
+    load 'v "('v,'r) exp" "('v,'r,'a) aux"
+  | store 'v "('v,'r) exp" "('v,'r,'a) aux"
+  | cas\<^sub>T 'v "('v,'r) exp" "('v,'r) exp" "('v,'r,'a) aux"
+  | cas\<^sub>F 'v "('v,'r) exp" "('v,'r) exp" "('v,'r,'a) aux"
   | op 'r "('v,'r) exp"
-  | test "('v,'r) exp" "'v \<Rightarrow> 'v \<Rightarrow> bool" "('v,'r) exp"
+  | cmp "('v,'r) exp" "'v \<Rightarrow> 'v \<Rightarrow> bool" "('v,'r) exp"
   | fence
   | cfence
   | stfence
+  | nop
 
 text \<open>Sub-Instruction Behaviour\<close>
-fun beh\<^sub>i :: "('v,'r) inst \<Rightarrow> ('v,'r) state rel"
+fun beh\<^sub>i :: "('v,'r,'a) inst \<Rightarrow> ('v,'r,'a) tstate_scheme rel"
   where
-    "beh\<^sub>i (store addr e) = {(m,m'). m' = m (addr :=\<^sub>1 ev (snd m) e)}" |
-    "beh\<^sub>i (load addr e) = {(m,m'). m' = m \<and> ld m addr = ev (snd m) e}" |
-    "beh\<^sub>i (op r e) = {(m,m'). m' = m (r :=\<^sub>2 ev (snd m) e)}" |
-    "beh\<^sub>i (test e\<^sub>1 f e\<^sub>2) = {(m,m'). m = m' \<and> f (ev (snd m) e\<^sub>1) (ev (snd m) e\<^sub>2)}" |
+    "beh\<^sub>i (store a e f) = {(m,m'). m' = m (a :=\<^sub>s ev (rg m) e)} O {(m,m'). m' = more_update (\<lambda>x. f m) m}" |
+    "beh\<^sub>i (load a e f) = {(m,m'). m' = m \<and> st m a = ev (rg m) e} O {(m,m'). m' = more_update (\<lambda>x. f m) m}" |
+    "beh\<^sub>i (cas\<^sub>T a e\<^sub>1 e\<^sub>2 f) = {(m,m'). m' = m (a :=\<^sub>s ev (rg m) e\<^sub>2) \<and> st m a = ev (rg m) e\<^sub>1} O {(m,m'). m' = more_update (\<lambda>x. f m) m}" |
+    "beh\<^sub>i (cas\<^sub>F a e\<^sub>1 e\<^sub>2 f) = {(m,m'). m' = m \<and> st m a \<noteq> ev (rg m) e\<^sub>1} O {(m,m'). m' = more_update (\<lambda>x. f m) m}" |
+    "beh\<^sub>i (op r e) = {(m,m'). m' = m (r :=\<^sub>r ev (rg m) e)}" |
+    "beh\<^sub>i (cmp e\<^sub>1 f e\<^sub>2) = {(m,m'). m = m' \<and> f (ev (rg m) e\<^sub>1) (ev (rg m) e\<^sub>2)}" |
     "beh\<^sub>i _ = Id"
 
+fun mems
+  where 
+    "mems (load y _ _) = {y}" |
+    "mems (store y _ _) = {y}" |
+    "mems (cas\<^sub>T y _ _ _) = {y}" |
+    "mems (cas\<^sub>F y _ _ _) = {y}" |
+    "mems _ = {}"
+
+fun wrs
+  where 
+    "wrs (op r _) = {r}" |
+    "wrs _ = {}"
+
+fun rds
+  where 
+    "rds (op _ e) = deps e" |
+    "rds (store _ e _) = deps e" |
+    "rds (load _ e _) = deps e" |
+    "rds (cas\<^sub>T _ e\<^sub>1 e\<^sub>2 _) = deps e\<^sub>1 \<union> deps e\<^sub>2" |
+    "rds (cas\<^sub>F _ e\<^sub>1 e\<^sub>2 _) = deps e\<^sub>1 \<union> deps e\<^sub>2" |
+    "rds _ = {}"
+
+fun addrs
+  where 
+    "addrs (op _ e) = addr e" |
+    "addrs (store _ e _) = addr e" |
+    "addrs (load _ e _) = addr e" |
+    "addrs (cas\<^sub>T _ e\<^sub>1 e\<^sub>2 _) = addr e\<^sub>1 \<union> addr e\<^sub>2" |
+    "addrs (cas\<^sub>F _ e\<^sub>1 e\<^sub>2 _) = addr e\<^sub>1 \<union> addr e\<^sub>2" |
+    "addrs _ = {}"
+
 text \<open>Sub-Instruction Reordering\<close>
-fun re\<^sub>i :: "('v,'r) inst \<Rightarrow> ('v,'r) inst \<Rightarrow> bool" 
+fun re\<^sub>i :: "('v,'r,'a) inst \<Rightarrow> ('v,'r,'a) inst \<Rightarrow> bool" 
   where
     "re\<^sub>i _ fence = False" |
     "re\<^sub>i fence _ = False" |
-    "re\<^sub>i (store _ _) stfence = False" |
-    "re\<^sub>i stfence (store _ _) = False" | 
-    "re\<^sub>i (test _ _ _) cfence = False" |
-    "re\<^sub>i cfence (load _ _) = False" |
-    "re\<^sub>i (load y _) (load x e) = (y \<noteq> x \<and> y \<notin> addrs e)" |
-    "re\<^sub>i (load y _) (store x e) = (y \<noteq> x \<and> y \<notin> addrs e)" |
-    "re\<^sub>i (load y e) (op r e') = (y \<notin> addrs e' \<and> r \<notin> deps e)" |
-    "re\<^sub>i (load y _) (test e\<^sub>1 _ e\<^sub>2) = (y \<notin> addrs e\<^sub>1 \<union> addrs e\<^sub>2)" |
-    "re\<^sub>i (store x _) (load y _) = (y \<noteq> x)" |
-    "re\<^sub>i (store x _) (store y _) = (y \<noteq> x)" |
-    "re\<^sub>i (store _ e) (op r _) = (r \<notin> deps e)" |
-    "re\<^sub>i (op r e) (op r' e') = (r \<notin> deps e' \<and> r' \<notin> deps e \<and> r \<noteq> r')" |
-    "re\<^sub>i (op r _) (test e\<^sub>1 _ e\<^sub>2) = (r \<notin> deps e\<^sub>1 \<and> r \<notin> deps e\<^sub>2)" |
-    "re\<^sub>i (op r _) (store _ e) = (r \<notin> deps e)" |
-    "re\<^sub>i (op r _) (load v e) = (r \<notin> deps e)" |
-    "re\<^sub>i (test _ _ _) (store _ _) = False" |
-    "re\<^sub>i (test e\<^sub>1 _ e\<^sub>2) (op r _) = (r \<notin> deps e\<^sub>1 \<and> r \<notin> deps e\<^sub>2)" |
-    "re\<^sub>i _ _ = True"
+    "re\<^sub>i (store _ _ _) stfence = False" |
+    "re\<^sub>i stfence (store _ _ _) = False" | 
+    "re\<^sub>i (cmp _ _ _) cfence = False" |
+    "re\<^sub>i cfence (load _ _ _) = False" |
+    "re\<^sub>i (cmp _ _ _) (store _ _ _) = False" |
+    "re\<^sub>i \<alpha> \<beta> = (mems \<alpha> \<inter> mems \<beta> = {} \<and> mems \<alpha> \<inter> addrs \<beta> = {} \<and> 
+                wrs \<alpha> \<inter> wrs \<beta> = {} \<and> rds \<alpha> \<inter> wrs \<beta> = {})"
 
 text \<open>Sub-Instruction Forwarding\<close>
-fun fwd\<^sub>i :: "('v,'r) inst \<Rightarrow> ('v,'r) inst \<Rightarrow> ('v,'r) inst" 
+fun fwd\<^sub>i :: "('v,'r,'a) inst \<Rightarrow> ('v,'r,'a) inst \<Rightarrow> ('v,'r,'a) inst" 
   where
-    "fwd\<^sub>i (load v\<^sub>a r\<^sub>a) (store v\<^sub>b r\<^sub>b) = (if v\<^sub>a = v\<^sub>b then test r\<^sub>a (=) r\<^sub>b else load v\<^sub>a r\<^sub>a)" |
-    "fwd\<^sub>i (store v\<^sub>a e) (op r e') = (store v\<^sub>a (subst e r e'))" |
-    "fwd\<^sub>i (load v\<^sub>a e) (op r e') = (load v\<^sub>a (subst e r e'))" |
-    "fwd\<^sub>i (test e\<^sub>1 f e\<^sub>2) (op r e) = (test (subst e\<^sub>1 r e) f (subst e\<^sub>2 r e))" |
+    "fwd\<^sub>i (load v\<^sub>a r\<^sub>a f) (store v\<^sub>b r\<^sub>b f') = (if v\<^sub>a = v\<^sub>b then cmp r\<^sub>a (=) r\<^sub>b else load v\<^sub>a r\<^sub>a f)" |
+    "fwd\<^sub>i (load v\<^sub>a r\<^sub>a f) (cas\<^sub>T v\<^sub>b _ e\<^sub>2 f') = (if v\<^sub>a = v\<^sub>b then cmp r\<^sub>a (=) e\<^sub>2 else load v\<^sub>a r\<^sub>a f)" |
+    "fwd\<^sub>i (store v\<^sub>a e f) (op r e') = (store v\<^sub>a (subst e r e') f)" |
+    "fwd\<^sub>i (load v\<^sub>a e f) (op r e') = (load v\<^sub>a (subst e r e') f)" |
+    "fwd\<^sub>i (cmp e\<^sub>1 f e\<^sub>2) (op r e) = (cmp (subst e\<^sub>1 r e) f (subst e\<^sub>2 r e))" |
     "fwd\<^sub>i (op r e) (op r' e') = (op r (subst e r' e'))" |
+    "fwd\<^sub>i (cas\<^sub>T v\<^sub>a e\<^sub>1 e\<^sub>2 f) (op r e) = (cas\<^sub>T v\<^sub>a (subst e\<^sub>1 r e) (subst e\<^sub>2 r e) f)" |
+    "fwd\<^sub>i (cas\<^sub>F v\<^sub>a e\<^sub>1 e\<^sub>2 f) (op r e) = (cas\<^sub>F v\<^sub>a (subst e\<^sub>1 r e) (subst e\<^sub>2 r e) f)" |
     "fwd\<^sub>i \<alpha> _ = \<alpha>"
 
 text \<open>Common Sub-Instructions\<close>
 
 abbreviation eq
-  where "eq r v \<equiv> test (Reg r) (=) (Val v)"
+  where "eq r v \<equiv> cmp (Reg r) (=) (Val v)"
 
 abbreviation assign
   where "assign r v \<equiv> op r (Exp (\<lambda>x. v) [])"
 
-abbreviation ntest
-  where "ntest e\<^sub>1 f e\<^sub>2 \<equiv> test e\<^sub>1 (\<lambda>x y. \<not> f x y) e\<^sub>2"
+abbreviation ncmp
+  where "ncmp e\<^sub>1 f e\<^sub>2 \<equiv> cmp e\<^sub>1 (\<lambda>x y. \<not> f x y) e\<^sub>2"
 
 section \<open>Sub-Instruction Specification Language\<close>
 
 text \<open>Wrap instructions in more abstract specification to facilitate verification\<close>
-type_synonym ('v,'r) ispec = "(('v,'r) inst,('v,'r) state) basic"
+type_synonym ('v,'r,'a) ispec = "(('v,'r,'a) inst, ('v,'r,'a) tstate_scheme) basic"
 
 text \<open>Duplicate forwarding and reordering behaviour of underlying instruction\<close>
-fun fwd\<^sub>s :: "('v,'r) ispec \<Rightarrow> ('v,'r) inst \<Rightarrow> ('v,'r) ispec" 
-  where "fwd\<^sub>s (\<alpha>,v,_) \<beta> =  (fwd\<^sub>i \<alpha> \<beta>,v,beh\<^sub>i (fwd\<^sub>i \<alpha> \<beta>))" 
+fun fwd\<^sub>s :: "('v,'r,'a) ispec \<Rightarrow> ('v,'r,'a) inst \<Rightarrow> ('v,'r,'a) ispec" 
+  where "fwd\<^sub>s (\<alpha>,v,_) \<beta> =  (fwd\<^sub>i \<alpha> \<beta>, v, beh\<^sub>i (fwd\<^sub>i \<alpha> \<beta>))" 
 
-abbreviation no_vc :: "('v,'r) inst \<Rightarrow> (('v,'r) inst,('v,'r) state) basic" ("\<lfloor>_\<rfloor>" 100)
+abbreviation no_vc :: "('v,'r,'a) inst \<Rightarrow> ('v,'r,'a) ispec" ("\<lfloor>_\<rfloor>" 100)
   where "no_vc \<alpha> \<equiv> (\<alpha>, UNIV, beh\<^sub>i \<alpha>)"
 
-abbreviation with_vc :: "('v,'r) pred \<Rightarrow> ('v,'r) inst \<Rightarrow> (('v,'r) inst,('v,'r) state) basic" ("\<lfloor>_,_\<rfloor>" 100)
+abbreviation with_vc :: "('v,'r,'a) pred \<Rightarrow> ('v,'r,'a) inst \<Rightarrow> ('v,'r,'a) ispec" ("\<lfloor>_,_\<rfloor>" 100)
   where "with_vc v \<alpha> \<equiv> (\<alpha>, Collect v, beh\<^sub>i \<alpha>)"
 
 section \<open>While Language Definition\<close>
-
-datatype ('v,'r) lang =
+datatype ('v,'r,'a) lang =
   Skip
-  | Load "('v,'r) pred" 'r 'r
-  | Store "('v,'r) pred" 'r 'r
-  | Op 'r "('v,'r) exp"
-  | Seq "('v,'r) lang" "('v,'r) lang"
-  | If "('v,'r) exp" "'v \<Rightarrow> 'v \<Rightarrow> bool" "('v,'r) exp" "('v,'r) lang" "('v,'r) lang"
-  | While "('v,'r) exp" "'v \<Rightarrow> 'v \<Rightarrow> bool" "('v,'r) exp" "('v,'r) pred" "('v,'r) lang"
+  | Fence
+  | Load "('v,'r,'a) pred" 'r 'r "('v,'r,'a) aux"
+  | Store "('v,'r,'a) pred" 'r 'r "('v,'r,'a) aux"
+  | Op 'r "('v,'r) exp" 
+  | CAS "('v,'r,'a) pred" 'r 'r 'r 'r 'v 'v "('v,'r,'a) aux"
+  | Seq "('v,'r,'a) lang" "('v,'r,'a) lang"
+  | If "('v,'r) exp" "'v \<Rightarrow> 'v \<Rightarrow> bool" "('v,'r) exp" "('v,'r,'a) lang" "('v,'r,'a) lang"
+  | While "('v,'r) exp" "'v \<Rightarrow> 'v \<Rightarrow> bool" "('v,'r) exp" "('v,'r,'a) pred" "('v,'r,'a) lang"
+  | DoWhile "('v,'r,'a) pred" "('v,'r,'a) lang" "('v,'r) exp" "'v \<Rightarrow> 'v \<Rightarrow> bool" "('v,'r) exp"
+  | Test "('v,'r,'a) pred"
+  | Assert "('v,'r,'a) pred"
 
 end
