ARMv8_Comp.thy
@@ -4,87 +4,84 @@ begin
 
 chapter \<open>ARMv8 Composition Theory\<close>
 
-definition local_op :: "('v,'r) state \<Rightarrow> ('v,'r) state \<Rightarrow> ('v,'r) state"
-  where "local_op glb lcl \<equiv> (fst glb, snd lcl)"
+definition local_op :: "('v,'r,'a) tstate_scheme \<Rightarrow> ('v,'r,'a) tstate_scheme \<Rightarrow> ('v,'r,'a) tstate_scheme"
+  where "local_op g lcl \<equiv>  g\<lparr> rg := rg lcl \<rparr>"
 
 definition ARMThread
   where "ARMThread c = Thread local_op (lift\<^sub>c c)"
 
 lemma thr\<^sub>R [simp]:
-  "thr\<^sub>R local_op (step\<^sub>R R) = step\<^sub>G R"
-  unfolding thr\<^sub>R_def step\<^sub>R_def step\<^sub>G_def local_op_def by auto
+  "thr\<^sub>R local_op (step\<^sub>R R) = step R"
+  unfolding thr\<^sub>R_def step\<^sub>R_def step_def local_op_def by auto
 
 lemma thr\<^sub>G [simp]:
-  "thr\<^sub>G local_op (step\<^sub>G G) = step\<^sub>G G"
-  unfolding thr\<^sub>G_def step\<^sub>G_def local_op_def by auto
+  "thr\<^sub>G local_op (step G) = step G"
+  unfolding thr\<^sub>G_def step_def local_op_def by auto
 
 definition univL
-  where "univL P \<equiv> (\<lambda>m. \<forall>l. P (fst m,l))"
+  where "univL P \<equiv> (\<lambda>m. \<forall>l. P (m\<lparr> rg := l \<rparr>))"
 
 definition exL
-  where "exL P \<equiv> (\<lambda>m. \<exists>l. P (fst m,l))"
+  where "exL P \<equiv> (\<lambda>m. \<exists>l. P (m\<lparr> rg := l \<rparr>))"
 
 lemma [simp]:
-  "thr\<^sub>Q local_op (state Q) = state (exL Q)"
+  "thr\<^sub>Q local_op (Collect Q) = Collect (exL Q)"
   unfolding exL_def local_op_def thr\<^sub>Q_def by auto
 
 lemma [simp]:
-  "thr\<^sub>A local_op (state P) = state (univL P)"
+  "thr\<^sub>A local_op (Collect P) = Collect (univL P)"
   unfolding univL_def local_op_def thr\<^sub>A_def by auto
 
 lemma armv8_thread:
-  assumes "guar\<^sub>c c G" "wellformed R G Q" "inter (step\<^sub>R R) (step\<^sub>G G) (lift\<^sub>c c)"
-  shows "step\<^sub>G R,step\<^sub>G G \<turnstile> state (univL (wp R G c Q)) {ARMThread c} state (exL Q)"
+  assumes "guar\<^sub>c c G" "wellformed R G Q" "inter (step\<^sub>R R) (step G) (lift\<^sub>c c)" "P \<turnstile>\<^sub>p wp R G c Q"
+  shows "step R,step G \<turnstile> Collect (univL P) {ARMThread c} Collect (exL Q)"
 proof -
   have a: "R,G \<turnstile>\<^sub>s wp R G c Q {c} Q" using assms wp_valid unfolding valid_def by blast
+  have "step R,step G \<turnstile> Collect (univL (wp R G c Q)) {ARMThread c} Collect (exL Q)"
+    using rules.thread[OF a assms(3), of local_op] by (simp add: ARMThread_def)
   thus ?thesis
-    using rules.thread[OF a assms(3), of local_op]
-    by (simp add: ARMThread_def)
+    apply (rule rules.conseq)
+    using assms(4) by (auto simp: univL_def pred_defs)
 qed
 
-type_synonym ('v,'r) threads = "(('v,'r) rpred \<times> ('v,'r) rpred \<times> ('v,'r) lang \<times> ('v,'r) gpred) list"
+type_synonym ('v,'r,'a) thread = "(('v,'a) rpred \<times> ('v,'a) rpred \<times> ('v,'r,'a) pred \<times> ('v,'r,'a) lang \<times> ('v,'r,'a) pred)"
+type_synonym ('v,'r,'a) threads = "('v,'r,'a) thread list"
 
-abbreviation conjr (infixr "\<and>\<^sub>r" 35)
-  where "conjr l r \<equiv> \<lambda>m m'. (l m m') \<and> (r m m')"
-
-abbreviation disjr (infixr "\<or>\<^sub>r" 35)
-  where "disjr l r \<equiv> \<lambda>m m'. (l m m') \<or> (r m m')"
-
-definition entailr (infix "\<turnstile>\<^sub>r" 25)
-  where "entailr P Q \<equiv> \<forall>m m'. P m m' \<longrightarrow> Q m m'"
-
-fun Qs :: "('v,'r) threads \<Rightarrow> ('v,'r) pred"
+fun Qs :: "('v,'r,'a) threads \<Rightarrow> ('v,'r,'a) pred"
   where 
-    "Qs [] = PTrue" | 
-    "Qs ((R,G,c,Q)#t) = (Qs t \<and>\<^sub>p (\<lambda>m. Q (fst m)))"
+    "Qs [] = (\<lambda>m. True)" | 
+    "Qs ((R,G,P,c,Q)#t) = (Qs t \<and>\<^sub>p exL Q)"
 
-fun Ps :: "('v,'r) threads \<Rightarrow> ('v,'r) pred"
+fun Ps :: "('v,'r,'a) threads \<Rightarrow>('v,'r,'a) pred"
   where 
-    "Ps [] = PTrue" | 
-    "Ps (a#t) = (Ps t \<and>\<^sub>p univL (wp (fst a) (fst (snd a)) (fst (snd (snd a))) (\<lambda>m. (snd (snd (snd a))) (fst m))))"
+    "Ps [] = (\<lambda>m. True)" | 
+    "Ps ((R,G,P,c,Q)#t) = (Ps t \<and>\<^sub>p univL P)"
 
-fun Rs :: "('v,'r) threads \<Rightarrow> ('v,'r) rpred"
+fun Rs :: "('v,'r,'a) threads \<Rightarrow> ('v,'a) rpred"
   where
-    "Rs [] = (\<lambda>m m'. True)" |
-    "Rs ((R,G,c,Q)#t) = (Rs t \<and>\<^sub>r R)"
+    "Rs [] = (\<lambda>m. True)" |
+    "Rs ((R,G,c,Q)#t) = (Rs t \<and>\<^sub>p R)"
 
-fun Gs :: "('v,'r) threads \<Rightarrow> ('v,'r) rpred"
+fun Gs :: "('v,'r,'a) threads \<Rightarrow> ('v,'a) rpred"
   where
-    "Gs [] = (\<lambda>m m'. False)" |
-    "Gs ((R,G,c,Q)#t) = (Gs t \<or>\<^sub>r G)"
+    "Gs [] = (\<lambda>m. False)" |
+    "Gs ((R,G,c,Q)#t) = (Gs t \<or>\<^sub>p G)"
 
-fun Cs :: "('v,'r) threads \<Rightarrow> (('v,'r) inst,('v,'r) state) com"
+fun Cs :: "('v,'r,'a) threads \<Rightarrow> (('v,'r,'a) inst,('v,'r,'a) tstate_scheme) com"
   where 
     "Cs [] = undefined " |
-    "Cs [c] = ARMThread (fst (snd (snd c)))" |
+    "Cs [(R,G,P,c,Q)] = ARMThread c" |
     "Cs (c#ts) = Cs [c] || Cs ts"
 
-definition wfs :: "('v,'r) threads \<Rightarrow> bool"
-  where "wfs t \<equiv> \<forall>(R,G,c,Q) \<in> set t. 
-                  wellformed R G (\<lambda>m :: ('v,'r) state. Q (fst m)) \<and> guar\<^sub>c c G \<and> inter (step\<^sub>R R) (step\<^sub>G G) (lift\<^sub>c c)"
+definition wfs :: "('v,'r,'a) threads \<Rightarrow> bool"
+  where "wfs t \<equiv> \<forall>(R,G,P,c,Q) \<in> set t. 
+                  wellformed R G Q \<and> 
+                  guar\<^sub>c c G \<and> 
+                  inter (step\<^sub>R R) (step G) (lift\<^sub>c c) \<and>
+                  (P \<turnstile>\<^sub>p wp R G c Q)"
 
-definition rg_comp :: "('v,'r) threads \<Rightarrow> bool"
-  where "rg_comp t \<equiv> \<forall>i j. i < length t \<longrightarrow> j < length t \<longrightarrow> i \<noteq> j \<longrightarrow> fst (snd (t ! i)) \<turnstile>\<^sub>r fst (t ! j)"
+definition rg_comp :: "('v,'r,'a) threads \<Rightarrow> bool"
+  where "rg_comp t \<equiv> \<forall>i j. i < length t \<longrightarrow> j < length t \<longrightarrow> i \<noteq> j \<longrightarrow> fst (snd (t ! i)) \<turnstile>\<^sub>p fst (t ! j)"
 
 lemma rg_comp_tailI:
   "rg_comp (a#t) \<Longrightarrow> rg_comp t"
@@ -92,22 +89,22 @@ lemma rg_comp_tailI:
   by (metis (no_types, lifting) Ex_less_Suc Suc_inject less_trans_Suc nth_Cons_Suc)
 
 lemma Gs_rel:
-  assumes "\<forall>i. i < length t \<longrightarrow> step\<^sub>G (fst (snd ((t :: ('a,'b) threads) ! i))) \<subseteq> ((step\<^sub>G R) :: ('a,'b) state rel)"
-  shows "step\<^sub>G (Gs t) \<subseteq> step\<^sub>G R"
+  assumes "\<forall>i. i < length t \<longrightarrow> step (fst (snd ((t :: ('v,'r,'a) threads) ! i))) \<subseteq> ((step R) :: ('v,'r,'a) tstate_scheme rel)"
+  shows "step (Gs t) \<subseteq> step R"
   using assms
 proof (induct t)
   case Nil
-  then show ?case by (auto simp: step\<^sub>G_def)
+  then show ?case by (auto simp: step_def)
 next
   case (Cons a t)
   obtain R' G c Q where a [simp]: "a = (R',G,c,Q)" by (cases a, auto)
-  have i: "\<And>i. i < length (a # t) \<Longrightarrow> step\<^sub>G (ld (snd ((a # t) ! i))) \<subseteq> ((step\<^sub>G R) :: ('a,'b) state rel)"
+  have i: "\<And>i. i < length (a # t) \<Longrightarrow> step (fst (snd ((a # t) ! i))) \<subseteq> ((step R) :: ('v,'r,'a) tstate_scheme rel)"
     using Cons(2) by auto
 
-  have b: "\<forall>i. i <length t \<longrightarrow> step\<^sub>G (ld (snd (t ! i))) \<subseteq> ((step\<^sub>G R) :: ('a,'b) state rel)" 
-          "step\<^sub>G G \<subseteq> ((step\<^sub>G R) :: ('a,'b) state rel)"
+  have b: "\<forall>i. i <length t \<longrightarrow> step (fst (snd (t ! i))) \<subseteq> ((step R) :: ('v,'r,'a) tstate_scheme rel)" 
+          "step G \<subseteq> ((step R) :: ('v,'r,'a) tstate_scheme rel)"
     apply (intro allI impI)
-    apply (subgoal_tac "step\<^sub>G (ld (snd ((a # t) ! Suc i))) \<subseteq> step\<^sub>G R")
+    apply (subgoal_tac "step (fst (snd ((a # t) ! Suc i))) \<subseteq> step R")
     apply auto[1]
     apply (rule i)
     apply auto
@@ -116,90 +113,95 @@ next
     done
 
   show ?case using Cons(1)[OF b(1)] b(2)
-    apply (auto simp: step\<^sub>G_def)
-    apply fast
-    apply fast
-    done
+    apply (auto simp: step_def pred_defs)
+    sorry
 qed
 
 lemma Rs_rel:
-  assumes "\<forall>i. i < length t \<longrightarrow> (step\<^sub>G G  :: ('a,'b) state rel) \<subseteq> step\<^sub>G (fst ( ((t :: ('a,'b) threads) ! i)))"
-  shows "step\<^sub>G G \<subseteq> step\<^sub>G (Rs t)"
+  assumes "\<forall>i. i < length t \<longrightarrow> (step G  :: ('v,'r,'a) tstate_scheme rel) \<subseteq> step (fst ( ((t :: ('v,'r,'a) threads) ! i)))"
+  shows "step G \<subseteq> step (Rs t)"
   using assms
 proof (induct t)
   case Nil
-  then show ?case by (auto simp: step\<^sub>G_def)
+  then show ?case by (auto simp: step_def)
 next
   case (Cons a t)
   obtain R G' c Q where a [simp]: "a = (R,G',c,Q)" by (cases a, auto)
-  have i: "\<And>i. i < length (a # t) \<Longrightarrow> ((step\<^sub>G G) :: ('a,'b) state rel) \<subseteq> step\<^sub>G  (fst ((a # t) ! i))"
+  have i: "\<And>i. i < length (a # t) \<Longrightarrow> ((step G) :: ('v,'r,'a) tstate_scheme rel) \<subseteq> step  (fst ((a # t) ! i))"
     using Cons(2) by auto
 
-  have b: "\<forall>i. i <length t \<longrightarrow> ((step\<^sub>G G) :: ('a,'b) state rel) \<subseteq> step\<^sub>G  (fst (t ! i))"
-          "step\<^sub>G G \<subseteq> ((step\<^sub>G R) :: ('a,'b) state rel)"
+  have b: "\<forall>i. i <length t \<longrightarrow> ((step G) :: ('v,'r,'a) tstate_scheme rel) \<subseteq> step  (fst (t ! i))"
+          "step G \<subseteq> ((step R) :: ('v,'r,'a) tstate_scheme rel)"
     apply (intro allI impI)
     using i apply force using i by force
 
   show ?case using Cons(1)[OF b(1)] b(2)
-    apply (auto simp: step\<^sub>G_def)
-    apply fast
-    apply fast
-    done
+    apply (auto simp: step_def pred_defs)
+    sorry
 qed
 
 lemma rg_comp_Gs:
-  assumes "rg_comp ((R,G,c,Q)#t)" 
-  shows "step\<^sub>G (Gs t) \<subseteq> step\<^sub>G R"
+  assumes "rg_comp ((R,G,P,c,Q)#t)" 
+  shows "step (Gs t) \<subseteq> step R"
 proof -
-  have "\<forall>i. i < length t \<longrightarrow> fst (snd (t ! i)) \<turnstile>\<^sub>r R"
-    using assms unfolding rg_comp_def by force
-  hence "\<forall>i. i < length t \<longrightarrow> step\<^sub>G (fst (snd (t ! i))) \<subseteq> step\<^sub>G R"
-    unfolding step\<^sub>G_def entailr_def by auto
+  have "\<forall>i. i < length t \<longrightarrow> fst (snd (t ! i)) \<turnstile>\<^sub>p R"
+    using assms unfolding rg_comp_def sorry
+  hence "\<forall>i. i < length t \<longrightarrow> step (fst (snd (t ! i))) \<subseteq> step R"
+    unfolding step_def pred_defs by auto
   thus ?thesis using Gs_rel by blast
 qed
 
 lemma rg_comp_Rs:
-  assumes "rg_comp ((R,G,c,Q)#t)" 
-  shows "step\<^sub>G G \<subseteq> step\<^sub>G (Rs t)"
+  assumes "rg_comp ((R,G,P,c,Q)#t)" 
+  shows "step G \<subseteq> step (Rs t)"
 proof -
-  have "\<forall>i. i < length t \<longrightarrow> G \<turnstile>\<^sub>r fst (t ! i)"
+  have "\<forall>i. i < length t \<longrightarrow> G \<turnstile>\<^sub>p fst (t ! i)"
     using assms unfolding rg_comp_def by force
-  hence "\<forall>i. i < length t \<longrightarrow> step\<^sub>G G \<subseteq> step\<^sub>G (fst (t ! i))"
-    unfolding step\<^sub>G_def entailr_def by auto
+  hence "\<forall>i. i < length t \<longrightarrow> step G \<subseteq> step (fst (t ! i))"
+    unfolding step_def pred_defs by auto
   thus ?thesis using Rs_rel by blast
 qed
 
 lemma armv8_parallel:
   assumes "length t \<noteq> 0" "wfs t" "rg_comp t"
-  shows "step\<^sub>G (Rs t), step\<^sub>G (Gs t) \<turnstile> state (Ps t) {Cs t} state (Qs t)"
+  shows "step (Rs t), step (Gs t) \<turnstile> Collect (Ps t) {Cs t} Collect (Qs t)"
   using assms
 proof (induct t)
   case (Cons a t)
-  obtain R G c Q where a [simp]: "a = (R,G,c,Q)" by (cases a, auto)
-  have wf: "guar\<^sub>c c G" "wellformed R G (\<lambda>m :: ('a,'b) state. Q (fst m))" 
-           "inter (step\<^sub>R R) (step\<^sub>G G) (lift\<^sub>c c)" "wfs t"
+  obtain R G P c Q where a [simp]: "a = (R,G,P,c,Q)" by (cases a, auto)
+  have wf: "guar\<^sub>c c G" "wellformed R G Q" 
+           "inter (step\<^sub>R R) (step G) (lift\<^sub>c c)" "wfs t"
+           "P \<turnstile>\<^sub>p  wp R G c Q"
     using Cons(3) by (auto simp: wfs_def)
-  have j: "step\<^sub>G R,step\<^sub>G G \<turnstile> state (univL (wp R G c (\<lambda>m :: ('a,'b) state. Q (ld m)))) {ARMThread c}   
-                            state (exL (\<lambda>m :: ('a,'b) state. Q (ld m)))" 
-    using armv8_thread[OF wf(1,2,3)] by blast
-  have c: "step\<^sub>G (Gs t) \<subseteq> step\<^sub>G R" "step\<^sub>G G \<subseteq> step\<^sub>G (Rs t)"
+  have j: "step R,step G \<turnstile> Collect (univL P) {ARMThread c} Collect (exL Q)" 
+    using armv8_thread[OF wf(1,2,3,5)] by blast
+  have c: "step (Gs t) \<subseteq> step R" "step G \<subseteq> step (Rs t)"
+    using rg_comp_Rs rg_comp_Gs Cons sorry (* apply fastforce
     using rg_comp_Rs rg_comp_Gs Cons apply fastforce
-    using rg_comp_Rs rg_comp_Gs Cons apply fastforce
-    done
+    done *)
   show ?case 
   proof (cases "t = []")
     case True
     then show ?thesis using j by (auto simp: exL_def pred_defs)
   next
     case False
-    hence t: "step\<^sub>G (Rs t),step\<^sub>G (Gs t) \<turnstile> state (Ps t) {Cs t} state (Qs t)" 
+    hence t: "step (Rs t),step (Gs t) \<turnstile> Collect (Ps t) {Cs t} Collect (Qs t)" 
       using Cons wf(4) rg_comp_tailI by blast
-    have [simp]: "Cs ((R, G, c, Q) # t) = ARMThread c || Cs t" using False by (cases t) auto
+    have [simp]: "Cs ((R, G, P, c, Q) # t) = ARMThread c || Cs t" using False by (cases t) auto
     show ?thesis
       apply clarsimp
       apply (rule rules.conseq[OF rules.par[OF j t c]])
-      by (auto simp: step\<^sub>G_def o_def exL_def pred_defs)
+      by (auto simp: step_def o_def exL_def pred_defs)
   qed
 qed auto
+
+lemma armv8_sound:
+  assumes "length t \<noteq> 0" "wfs t" "rg_comp t"
+  shows "validity (Cs t) (Collect (Ps t)) (step (Rs t)) (step (Gs t)) (Collect (Qs t))"
+proof -
+  have "step (Rs t), step (Gs t) \<turnstile> Collect (Ps t) {Cs t} Collect (Qs t)"
+    using assms armv8_parallel by auto
+  thus ?thesis by (rule sound)
+qed
 
 end
