ARMv8_State.thy
@@ -1,0 +1,86 @@
+theory ARMv8_State
+  imports Main
+begin
+
+
+section \<open>State Encoding\<close>
+
+record 'v gstate = st :: "'v \<Rightarrow> 'v"
+record ('v,'r) tstate = "'v gstate" + rg :: "'r \<Rightarrow> 'v"
+type_synonym ('v,'r,'a) pred = "('v,'r,'a) tstate_scheme \<Rightarrow> bool"
+type_synonym ('v,'a) rpred = "(('v,'a) gstate_scheme \<times> ('v,'a) gstate_scheme) \<Rightarrow> bool"
+
+
+
+(*
+type_synonym ('v) global = "(('v \<Rightarrow> 'v))"
+type_synonym ('v,'r) state = "(('v) global \<times> ('r \<Rightarrow> 'v))"
+type_synonym ('v,'r) rpred = "(('v) global \<times> ('v) global) \<Rightarrow> bool"
+type_synonym ('v,'r) gpred  = "('v) global \<Rightarrow> bool"
+*)
+
+
+section \<open>Write Operations\<close>
+
+definition st_upd :: "(('v,'a) gstate_scheme) \<Rightarrow> 'v \<Rightarrow> 'v \<Rightarrow> (('v,'a) gstate_scheme)"
+  where "st_upd f a b = f \<lparr> st := ((st f) (a := b)) \<rparr>"
+
+definition rg_upd :: "(('v,'r,'a) tstate_scheme) \<Rightarrow> 'r \<Rightarrow> 'v \<Rightarrow> (('v,'r,'a) tstate_scheme)"
+  where "rg_upd f a b = f \<lparr> rg := ((rg f) (a := b)) \<rparr>"
+
+nonterminal updbinds and updbind
+
+syntax
+  "_updbindm" :: "'a \<Rightarrow> 'a \<Rightarrow> updbind"             ("(2_ :=\<^sub>s/ _)")
+  "_updbindr" :: "'a \<Rightarrow> 'a \<Rightarrow> updbind"             ("(2_ :=\<^sub>r/ _)")
+  ""         :: "updbind \<Rightarrow> updbinds"             ("_")
+  "_updbinds":: "updbind \<Rightarrow> updbinds \<Rightarrow> updbinds" ("_,/ _")
+  "_Update"  :: "'a \<Rightarrow> updbinds \<Rightarrow> 'a"            ("_/'((_)')" [1000, 0] 900)
+
+translations
+  "_Update f (_updbinds b bs)" \<rightleftharpoons> "_Update (_Update f b) bs"
+  "f(x:=\<^sub>ry)" \<rightleftharpoons> "CONST rg_upd f x y"
+  "f(x:=\<^sub>sy)" \<rightleftharpoons> "CONST st_upd f x y"
+
+section \<open>Simple Predicate Encoding\<close>
+
+named_theorems pred_defs
+
+definition conj  (infixr "\<and>\<^sub>p" 35)
+  where "conj l r \<equiv> \<lambda>m. (l m) \<and> (r m)"
+
+definition disj  (infixr "\<or>\<^sub>p" 35)
+  where "disj l r \<equiv> \<lambda>m. (l m) \<or> (r m)"
+
+definition imp  (infixr "\<longrightarrow>\<^sub>p" 35)
+  where "imp l r \<equiv> \<lambda>m. (l m) \<longrightarrow> (r m)"
+
+definition entail (infix "\<turnstile>\<^sub>p" 25)
+  where "entail P Q \<equiv> \<forall>m. P m \<longrightarrow> Q m"
+
+definition assert
+  where "assert b \<equiv> \<lambda>m. b"
+
+declare conj_def [pred_defs]
+declare disj_def [pred_defs]
+declare imp_def [pred_defs]
+declare assert_def [pred_defs]
+declare entail_def [pred_defs]
+
+lemma [simp]:
+  "(P \<turnstile>\<^sub>p P) = True"
+  by (auto simp add: pred_defs)
+
+lemma [simp]:
+  "(P \<and>\<^sub>p P) = P"
+  by (auto simp: pred_defs)
+
+section \<open>Base Definitions for Relations\<close>
+
+definition reflexive 
+  where "reflexive R \<equiv> \<forall>m . R (m,m)"
+
+definition transitive 
+  where "transitive R \<equiv> \<forall>m m' m''. R (m,m') \<longrightarrow> R (m',m'') \<longrightarrow> R (m,m'')"
+
+end
